Weidenbach_Book/IsaSAT/IsaSAT_ACIDS.thy
@@ -1,7 +1,6 @@
 ﻿theory IsaSAT_ACIDS
   imports IsaSAT_Literals
-    IsaSAT_VSIDS
-    Pairing_Heaps
+    Heaps_Abs
 begin
 text \<open>Instead of using VSIDS (which requires float), we use the more stable ACIDS variant
   that works simply on integers and does not seem much worse.
@@ -12,7 +11,135 @@ integer, we simply stop incrementing it. \<close>
 (*TODO rename VSIDS to ACIDS even if the difference is simply the bumping score*)
 section \<open>ACIDS\<close>
 
-definition acids :: \<open>'a multiset \<Rightarrow> ('a, 'ann) ann_lits \<Rightarrow> 'a multiset \<times> ('a \<Rightarrow> 'v) \<times> 'v :: linorder \<Rightarrow> bool\<close> where
-\<open>acids \<A> M = (\<lambda>(b, w, m). b \<subseteq># \<A> \<and> Max (w ` set_mset \<A>) \<le> m \<and> (\<forall>L \<in>#\<A>. L \<notin># b \<longrightarrow> defined_lit M (Pos L)))\<close>
-thm VSIDS.mop_prio_peek_min_def
+type_synonym ('a, 'v) acids = \<open>('a multiset \<times> ('a multiset \<times> ('a \<Rightarrow> 'v)) \<times> 'v)\<close>
+definition acids :: \<open>'a multiset \<Rightarrow> ('a, 'ann) ann_lits \<Rightarrow> ('a, 'v::linorder) acids set\<close> where
+\<open>acids \<A> M = {(\<B>, (b, w), m). \<B> = \<A> \<and> b \<subseteq># \<A> \<and> Max (w ` set_mset \<A>) \<le> m \<and> (\<forall>L \<in>#\<A>. L \<notin># b \<longrightarrow> defined_lit M (Pos L)) \<and> distinct_mset b}\<close>
+
+lemma acids_prepend: \<open>ac \<in> acids \<A> M \<Longrightarrow> ac \<in> acids \<A> (L # M)\<close>
+  unfolding acids_def by (auto simp: defined_lit_map)
+
+interpretation ACIDS: hmstruct_with_prio where
+  le = \<open>(\<ge>) :: nat \<Rightarrow> nat \<Rightarrow> bool\<close> and
+  lt = \<open>(>)\<close>
+  apply unfold_locales
+  subgoal by auto
+  subgoal by auto
+  subgoal by (auto simp: transp_def)
+  subgoal by (auto simp: totalp_on_def)
+  done
+
+definition acids_tl :: \<open>'a \<Rightarrow> ('a, 'v) acids \<Rightarrow> ('a, 'v) acids nres\<close> where
+  \<open>acids_tl L = (\<lambda>(\<B>, ac, m). do {
+    ASSERT (L \<in># \<B>);
+    ac \<leftarrow> ACIDS.mop_prio_insert_unchanged L ac;
+    RETURN (\<B>, ac, m)
+  })\<close>
+
+lemma acids_tl:
+  \<open>ac \<in> acids \<A> M \<Longrightarrow> L \<in># \<A> \<Longrightarrow> M \<noteq> [] \<Longrightarrow> L = atm_of (lit_of (hd M)) \<Longrightarrow> acids_tl L ac \<le> RES (acids \<A> (tl M))\<close>
+  unfolding acids_tl_def ACIDS.mop_prio_insert_unchanged_def
+    ACIDS.mop_prio_insert_raw_unchanged_def
+  apply refine_vcg
+  subgoal
+    by (cases M) (auto simp: acids_def ACIDS.mop_prio_insert_unchanged_def insert_subset_eq_iff
+      intro!: subset_add_mset_notin_subset)
+  subgoal
+    apply (cases M)
+    apply (auto simp: acids_def ACIDS.mop_prio_insert_unchanged_def
+      defined_lit_map)
+    using insert_subset_eq_iff subset_add_mset_notin_subset by fastforce
+  done
+
+definition acids_get_min :: \<open>('a, nat) acids \<Rightarrow> 'a nres\<close> where
+  \<open>acids_get_min = (\<lambda>(\<B>, ac, m). do {
+    L \<leftarrow> ACIDS.mop_prio_peek_min ac;
+    RETURN L
+  })\<close>
+
+definition acids_mset where
+  \<open>acids_mset x = fst (fst (snd x))\<close>
+
+lemma acids_get_min:
+  \<open>acids_mset x \<noteq> {#} \<Longrightarrow> acids_get_min x \<le> SPEC (\<lambda>v. ACIDS.prio_peek_min (fst (snd x)) v)\<close>
+  unfolding acids_get_min_def ACIDS.mop_prio_peek_min_def acids_mset_def
+  by refine_vcg (auto simp: ACIDS.prio_peek_min_def)
+
+definition acids_pop_min :: \<open>('a, nat) acids \<Rightarrow> ('a \<times> ('a, nat) acids) nres\<close> where
+  \<open>acids_pop_min = (\<lambda>(\<B>, ac, m). do {
+    (v, ac) \<leftarrow> ACIDS.mop_prio_pop_min ac;
+    RETURN (v, (\<B>, ac, m))
+  })\<close>
+
+definition acids_find_next_undef :: \<open>nat multiset \<Rightarrow> (nat, nat) acids \<Rightarrow> (nat, nat) ann_lits \<Rightarrow> (nat option \<times> (nat, nat) acids) nres\<close> where
+\<open>acids_find_next_undef \<A> = (\<lambda>ac M. do {
+  WHILE\<^sub>T\<^bsup>(\<lambda>(L, ac).
+        (L = None \<longrightarrow> ac \<in> acids \<A> M) \<and>
+        (L \<noteq> None \<longrightarrow> ac \<in> acids \<A> (Decided (Pos (the L)) # M) \<and> Pos (the L) \<in># \<L>\<^sub>a\<^sub>l\<^sub>l \<A> \<and> undefined_lit M (Pos (the L))))
+  \<^esup>
+      (\<lambda>(nxt, ac). nxt = None \<and> acids_mset ac \<noteq> {#})
+      (\<lambda>(a, ac). do {
+         ASSERT (a = None);
+         (L, ac) \<leftarrow> acids_pop_min ac;
+         ASSERT(Pos L \<in># \<L>\<^sub>a\<^sub>l\<^sub>l  \<A>);
+         if defined_lit M (Pos L) then RETURN (None, ac)
+         else RETURN (Some L, ac)
+        }
+      )
+      (None, ac)
+  })\<close>
+
+lemma acids_pop_min:
+  \<open>acids_mset x \<noteq> {#} \<Longrightarrow> x \<in> acids \<A> M \<Longrightarrow>
+  acids_pop_min x \<le> SPEC (\<lambda>(v, ac). acids_mset ac = acids_mset x - {#v#} \<and> v \<in># acids_mset x \<and>
+    ACIDS.prio_peek_min (fst (snd x)) v \<and>
+    (defined_lit M (Pos v) \<longrightarrow> ac \<in> acids \<A> M) \<and>
+    (undefined_lit M (Pos v) \<longrightarrow> ac \<in> acids \<A> (Decided (Pos v) # M)))\<close>
+  unfolding ACIDS.mop_prio_pop_min_def acids_pop_min_def
+    ACIDS.mop_prio_peek_min_def ACIDS.mop_prio_del_def
+  by refine_vcg
+   (auto simp: acids_def ACIDS.prio_peek_min_def distinct_mset_remove1_All ACIDS.prio_del_def
+      defined_lit_map acids_mset_def dest: in_diffD)
+
+lemma acids_find_next_undef:
+  assumes
+    vmtf: \<open>ac \<in> acids \<A> M\<close>
+  shows \<open>acids_find_next_undef \<A> ac M
+     \<le> \<Down> Id (SPEC (\<lambda>(L, ac).
+        (L = None \<longrightarrow> ac \<in> acids \<A> M \<and> (\<forall>L\<in>#\<L>\<^sub>a\<^sub>l\<^sub>l \<A>. defined_lit M L)) \<and>
+        (L \<noteq> None \<longrightarrow> ac \<in> acids \<A> (Decided (Pos (the L)) # M) \<and> Pos (the L) \<in># \<L>\<^sub>a\<^sub>l\<^sub>l \<A> \<and> undefined_lit M (Pos (the L)))))\<close>
+proof -
+  have [refine0]: \<open>wf (measure (\<lambda>(_, ac). size (acids_mset ac)))\<close>
+    by auto
+  show ?thesis
+    unfolding acids_find_next_undef_def
+    apply (refine_vcg acids_pop_min[of _ \<A> M, THEN order_trans])
+    subgoal using assms by auto
+    subgoal by auto
+    subgoal by (auto simp: ACIDS.prio_peek_min_def acids_def acids_mset_def
+      in_\<L>\<^sub>a\<^sub>l\<^sub>l_atm_of_\<A>\<^sub>i\<^sub>n)
+    subgoal by auto
+    subgoal by auto
+    subgoal by auto
+    subgoal by auto
+    subgoal by (auto simp: acids_def ACIDS.prio_peek_min_def
+      in_\<L>\<^sub>a\<^sub>l\<^sub>l_atm_of_\<A>\<^sub>i\<^sub>n)
+    subgoal by auto
+    subgoal by auto
+    subgoal by auto
+    subgoal by auto
+    subgoal by (auto simp: ACIDS.prio_peek_min_def acids_mset_def dest: multi_member_split)
+    subgoal by auto
+    subgoal by auto
+    subgoal by auto
+    subgoal by auto
+    subgoal by (auto simp: ACIDS.prio_peek_min_def acids_mset_def dest: multi_member_split)
+    subgoal by auto
+    subgoal by (auto simp: ACIDS.prio_peek_min_def acids_mset_def acids_def
+      in_\<L>\<^sub>a\<^sub>l\<^sub>l_atm_of_\<A>\<^sub>i\<^sub>n dest!: multi_member_split[of \<open>_ :: nat\<close>])
+    subgoal by auto
+    subgoal by auto
+    subgoal by auto
+    done
+qed
+
 end
